Define a simple initial state that inits the globals
Summary:
Global variables need allocating and initialising before the machine can
start. The definition here shouldn't constrain how and where they are
allocated. For example, they don't all need to have separate
allocations. We also tag allocated blocks so that the allocation for a
global can never be deallocated.

Start working on a sanity checking invariant on states.

Reviewed By: jberdine

Differential Revision: D16735068

fbshipit-source-id: 0d5e60e7a

sledge/semantics/llvmScript.sml
@@ -110,6 +110,14 @@ Datatype `
 
 type_abbrev ("prog", ``:fun_name |-> def``);
 
+Definition terminator_def:
+  (terminator (Ret _) ⇔ T) ∧
+  (terminator (Br _ _ _) ⇔ T) ∧
+  (terminator (Invoke _ _ _ _ _ _) ⇔ T) ∧
+  (terminator Unreachable ⇔ T) ∧
+  (terminator _ ⇔ F)
+End
+
 (* ----- Semantic states ----- *)
 
 Datatype `
@@ -137,10 +145,13 @@ Datatype `
 Datatype `
   state =
     <| ip : pc;
-       globals : glob_var |-> word64;
+       (* Keep the size of the global with its memory address *)
+       globals : glob_var |-> (num # word64);
        locals : loc_var |-> pv;
        stack : frame list;
-       allocations : (num # num) set;
+       (* The set of allocated ranges. The bool indicates whether the range is
+        * free-able or not *)
+       allocations : (bool # num # num) set;
        heap : addr |-> bool # word8 |>`;
 
 (* ----- Things about types ----- *)
@@ -255,7 +266,7 @@ Definition eval_const_def:
   (eval_const g (GlobalC var) =
     case flookup g var of
     | None => PtrV 0w
-    | Some w => PtrV w) ∧
+    | Some (s,w) => PtrV w) ∧
   (eval_const g UndefC = UndefV)
 Termination
   WF_REL_TAC `measure (const_size o snd)` >> rw [listTheory.MEM_MAP] >>
@@ -292,12 +303,12 @@ Definition inc_pc_def:
 End
 
 Definition interval_to_set_def:
-  interval_to_set (start,stop) =
+  interval_to_set (_, start,stop) =
     { n | start ≤ n ∧ n < stop }
 End
 
 Definition interval_ok_def:
-  interval_ok (i1, i2) ⇔
+  interval_ok (_, i1, i2) ⇔
     i1 ≤ i2 ∧ i2 < 2 ** 64
 End
 
@@ -315,7 +326,7 @@ End
 
 Inductive allocate:
   (v2n v.value = Some m ∧
-   b = (w2n w, w2n w + m * len) ∧
+   b = (T, w2n w, w2n w + m * len) ∧
    is_free b s.allocations
    ⇒
    allocate s v len
@@ -325,15 +336,15 @@ End
 
 Definition deallocate_def:
   (deallocate (A n) (Some allocs) =
-    if ∃m. (n,m) ∈ allocs then
-      Some { (start,stop) | (start,stop) ∈ allocs ∧ start ≠ n }
+    if ∃m. (T,n,m) ∈ allocs then
+      Some { (b,start,stop) | (b,start,stop) ∈ allocs ∧ start ≠ n }
     else
       None) ∧
   (deallocate _ None = None)
 End
 
 Definition get_bytes_def:
-  get_bytes h (start, stop) =
+  get_bytes h (_, start, stop) =
     map
       (λoff.
         case flookup h (A (start + off)) of
@@ -531,7 +542,7 @@ Inductive step_instr:
      (inc_pc (update_result r v2 s2))) ∧
 
   (eval s a1 = <| poison := p1; value := PtrV w |> ∧
-   interval = (w2n w, w2n w + sizeof t) ∧
+   interval = (b, w2n w, w2n w + sizeof t) ∧
    is_allocated interval s.allocations ∧
    pbytes = get_bytes s.heap interval
    ⇒
@@ -542,7 +553,7 @@ Inductive step_instr:
                             s))) ∧
 
   (eval s a2 = <| poison := p2; value := PtrV w |> ∧
-   interval = (w2n w, w2n w + sizeof t) ∧
+   interval = (b, w2n w, w2n w + sizeof t) ∧
    is_allocated interval s.allocations ∧
    bytes = value_to_bytes (eval s a1).value ∧
    length bytes = sizeof t
@@ -613,14 +624,90 @@ Inductive next_instr:
   flookup d.blocks s.ip.b = Some b ∧ 
   s.ip.i < length b.body
   ⇒
-  next_instr p (el s.ip.i b.body)
+  next_instr p s (el s.ip.i b.body)
 End
 
 Inductive step:
-  next_instr p i ∧
+  next_instr p s i ∧
   step_instr p s i s'
   ⇒
   step p s s'
+End
+
+(* ----- Initial state ----- *)
+
+Definition allocations_ok_def:
+  allocations_ok s ⇔
+    ∀i1 i2.
+      i1 ∈ s.allocations ∧ i2 ∈ s.allocations
+      ⇒
+      interval_ok i1 ∧ interval_ok i2 ∧
+      (interval_to_set i1 ∩ interval_to_set i2 ≠ ∅ ⇒
+       interval_to_set i1 = interval_to_set i2)
+End
+
+Definition heap_ok_def:
+  heap_ok s ⇔
+    ∀i n. i ∈ s.allocations ∧ n ∈ interval_to_set i ⇒ flookup s.heap (A n) ≠ None
+End
+
+Definition globals_ok_def:
+  globals_ok s ⇔
+    ∀g n w.
+      flookup s.globals g = Some (n, w)
+      ⇒
+      is_allocated (F, w2n w, w2n w + n) s.allocations
+End
+
+(* The initial state contains allocations for the initialised global variables *)
+Definition is_init_state_def:
+  is_init_state s (global_init : glob_var |-> ty # v) ⇔
+    s.ip.f = Fn "main" ∧
+    s.ip.b = None ∧
+    s.ip.i = 0 ∧
+    s.locals = fempty ∧
+    s.stack = [] ∧
+    allocations_ok s ∧
+    globals_ok s ∧
+    fdom s.globals = fdom global_init ∧
+    s.allocations ⊆ {F, start, stop | T} ∧
+    ∀g w t v n.
+      flookup s.globals g = Some (n, w) ∧ flookup global_init g = Some (t,v) ⇒
+      ∃bytes.
+        get_bytes s.heap (F, w2n w, w2n w + sizeof t) = map (λb. (F,b)) bytes ∧
+        bytes_to_value t bytes = (v, []) 
+End
+
+(* ----- Invariants on state ----- *)
+
+Definition prog_ok_def:
+  prog_ok p ⇔
+    ∀fname dec bname block.
+      flookup p fname = Some dec ∧
+      flookup dec.blocks bname = Some block
+      ⇒
+      block.body ≠ [] ∧ terminator (last block.body)
+End
+
+Definition ip_ok_def:
+  ip_ok p ip ⇔
+    ∃dec block. flookup p ip.f = Some dec ∧ flookup dec.blocks ip.b = Some block ∧ ip.i < length block.body
+End
+
+Definition frame_ok_def:
+  frame_ok p s f ⇔
+    ip_ok p f.ret ∧
+    every (λn. ∃start stop. n = A start ∧ (T, start, stop) ∈ s.allocations) f.stack_allocs
+End    
+
+Definition stack_ok_def:
+  stack_ok p s ⇔
+    every (frame_ok p s) s.stack
+End
+
+Definition state_invariant_def:
+  state_invariant p s ⇔
+    ip_ok p s.ip ∧ allocations_ok s ∧ heap_ok s ∧ globals_ok s ∧ stack_ok p s
 End
 
 export_theory();
